lib/Extraction.v
@@ -1,7 +1,7 @@
 From Stdlib Require Import Bool List String PeanoNat.
 From Stdlib Require Import Extraction ExtrOcamlNativeString ExtrOcamlBasic ExtrOcamlNatInt.
 
-From lstar Require Import Lstar KV DFA TTT.
+From lstar Require Import Lstar KV Automata TTT.
 
 Extraction Language OCaml.
 
