theories/NLstar.v
@@ -1,0 +1,370 @@
+(** NL* RFSA learning
+    https://lsv.ens-paris-saclay.fr/Publis/RAPPORTS_LSV/PDF/rr-lsv-2008-28.pdf *)
+
+#[local] Set Warnings "-intuition-auto-with-star".
+
+From lstar Require Import Automata ListLemmas SetLemmas.
+From Stdlib Require Import List.
+From Stdlib Require Import Lia.
+From Stdlib Require Import PeanoNat.
+From Stdlib Require Import Setoids.Setoid.
+From Stdlib Require Import Eqdep_dec.
+Import ListNotations.
+From lstar Require Import Teacher.
+
+Module NLstar (s : Symbol) (L : ResidualLanguage s) (Tch : RFSATeacher s L).
+Import s L Tch N R.
+
+Definition mem := mem str_eq.
+
+Record hypothesis : Type := {
+  T  : str -> bool;
+  U  : list str;
+  V  : list str
+}.
+
+(** One-letter extensions of the access strings *)
+Definition USigma (o : hypothesis) : list str :=
+    flat_map (fun u => map (fun a => u ++ [a]) enum) o.(U).
+
+(** The strings indexing rows of the hypothesis: U together with U.Sigma *)
+Definition row_index (o : hypothesis) : list str :=
+    o.(U) ++ USigma o.
+
+(** The value of the row of u at column v *)
+Definition cell (o : hypothesis) (u v : str) : bool := o.(T) (u ++ v).
+
+(** Two rows are equal when they agree on every column *)
+Definition row_eq (o : hypothesis) (u1 u2 : str) : Prop :=
+    forall v, In v o.(V) -> cell o u1 v = cell o u2 v.
+
+(* Definition 5 *)
+(** The join of rows u1 u2 at column v *)
+Definition join (o : hypothesis) (u1 u2 v : str) : bool :=
+    cell o u1 v || cell o u2 v.
+
+(* Definition 6 *)
+(** A row r is composed when on every column its value is the join of rows
+    distinct from r among the row indices *)
+Definition composed (o : hypothesis) (u : str) : Prop :=
+    forall v, In v o.(V) ->
+        cell o u v = true <->
+        exists u', In u' (row_index o) /\ ~ row_eq o u' u /\ cell o u' v = true.
+
+(** If a row is not composed, it is prime *)
+Definition prime (o : hypothesis) (u : str) : Prop :=
+    In u (row_index o) /\ ~ composed o u.
+
+(* Definition 7 *)
+(** Row u1 is covered by row u2 when, on every column, a + in u1 forces a + in u2 *)
+Definition covered (o : hypothesis) (u1 u2 : str) : Prop :=
+    forall v, In v o.(V) -> cell o u1 v = true -> cell o u2 v = true.
+
+(** Row u1 is strictly covered by row u2 when it is covered and they differ
+    on some column *)
+Definition strictly_covered (o : hypothesis) (u1 u2 : str) : Prop :=
+    covered o u1 u2 /\ ~ row_eq o u1 u2.
+
+Lemma strict_impl_covered : forall o u1 u2,
+    strictly_covered o u1 u2 -> covered o u1 u2.
+Proof. intros. now destruct H. Qed.
+
+Lemma covered_dec : forall o u1 u2, {covered o u1 u2} + {~ covered o u1 u2}.
+Proof.
+    intros. unfold covered.
+    induction (V o).
+        left. intros. destruct H.
+    destruct (Bool.bool_dec (cell o u1 a) true).
+    - destruct (Bool.bool_dec (cell o u2 a) true).
+      + destruct IHl.
+            left. intros. destruct H; subst; auto.
+        right. intro. apply n. intros. apply H; auto. now right.
+      + right. intro. apply n. apply H; [now left | assumption].
+    - destruct IHl.
+        left. intros. destruct H; subst; [congruence | auto].
+      right. intro. apply n0. intros. apply H; auto. now right.
+Defined.
+
+Lemma row_eq_dec : forall o u1 u2, {row_eq o u1 u2} + {~ row_eq o u1 u2}.
+Proof.
+    intros. unfold row_eq.
+    induction (V o).
+        left. intros. destruct H.
+    destruct (Bool.bool_dec (cell o u1 a) (cell o u2 a)).
+    - destruct IHl.
+        left. intros. destruct H; subst; auto.
+      right. intro. apply n. intros. apply H. now right.
+    - right. intro. apply n, H. now left.
+Defined.
+
+Lemma strictly_covered_dec : forall o u1 u2,
+    {strictly_covered o u1 u2} + {~ strictly_covered o u1 u2}.
+Proof.
+    intros. unfold strictly_covered.
+    destruct (covered_dec o u1 u2).
+    - destruct (row_eq_dec o u1 u2).
+        right. now intros.
+      now left.
+    - right. now intros.
+Defined.
+
+Lemma composed_dec : forall o u, {composed o u} + {~ composed o u}.
+Proof.
+    intros. unfold composed.
+    induction (V o).
+        left. intros. destruct H.
+    assert (Pdec : {exists u', In u' (row_index o) /\ ~ row_eq o u' u /\ cell o u' a = true}
+                 + {~ exists u', In u' (row_index o) /\ ~ row_eq o u' u /\ cell o u' a = true}).
+    { clear IHl.
+        induction (row_index o).
+            right. intro Contra. destruct Contra, H. inversion H.
+        destruct (row_eq_dec o a0 u).
+        - destruct IHl0.
+            left. destruct e. exists x. intuition.
+          right. intro Contra. destruct Contra, H, H0. destruct H.
+            now subst.
+          apply n. exists x. auto.
+        - destruct (Bool.bool_dec (cell o a0 a) true).
+            left. exists a0. split; [now left | now split].
+          destruct IHl0.
+            left. destruct e. exists x. split; [now right | intuition].
+          right. intro Contra. destruct Contra, H, H0. destruct H.
+            now subst.
+          apply n1. exists x. auto.
+    }
+    destruct (Bool.bool_dec (cell o u a) true).
+    - destruct Pdec.
+      + destruct IHl.
+            left. intros. destruct H; [subst; now split | auto].
+        right. intro. apply n. intros. apply H. now right.
+      + right. intro. apply n. now apply (proj1 (H a (or_introl eq_refl))).
+    - destruct Pdec.
+        right. intro. apply n. now apply (proj2 (H a (or_introl eq_refl))).
+      destruct IHl.
+        left. intros. destruct H.
+            subst. intuition.
+        now apply i.
+      right. intro. apply n1. intros. apply H. now right.
+Defined.
+
+Lemma prime_dec : forall o u, {prime o u} + {~ prime o u}.
+Proof.
+    intros. unfold prime.
+    destruct (in_dec str_eq u (row_index o)).
+    - destruct (composed_dec o u).
+        right. now intros (_ & ?).
+      left. now split.
+    - right. now intros (? & _).
+Defined.
+
+Lemma composed_prime_dec : forall o u,
+    In u (row_index o) -> {composed o u} + {prime o u}.
+Proof.
+    intros. destruct (composed_dec o u).
+        now left.
+    right. now split.
+Defined.
+
+Definition prime_reps (o : hypothesis) : list str :=
+    filter (fun u => if prime_dec o u then true else false) (row_index o).
+
+Lemma prime_reps_prime : forall o u, In u (prime_reps o) -> prime o u.
+Proof.
+    intros. apply filter_In in H. destruct H. now destruct (prime_dec o u).
+Qed.
+
+Lemma prime_reps_index : forall o u, In u (prime_reps o) -> In u (row_index o).
+Proof.
+    intros. apply filter_In in H. now destruct H.
+Qed.
+
+Definition memr (o : hypothesis) (q : str) : bool := mem q (prime_reps o).
+
+Definition cover_set (o : hypothesis) (u : str) : list str :=
+    filter (fun p => if covered_dec o p u then true else false) (prime_reps o).
+
+Lemma cover_set_prime_reps : forall o u p,
+    In p (cover_set o u) -> In p (prime_reps o).
+Proof.
+    intros. apply filter_In in H. now destruct H.
+Qed.
+
+Lemma cover_set_memr : forall o u p,
+    In p (cover_set o u) -> memr o p = true.
+Proof.
+    intros. now apply mem_In, (cover_set_prime_reps o u).
+Qed.
+
+(* Definition 8 *)
+(** A table is RFSA-closed if, for each r \in Rows_low(T),
+    r = fold Union {r' \in Primes_upper(T) | r' covered by r} *)
+
+(** The closedness condition for a single lower row u: on every column, u's
+    value is the join of the prime upper rows covered by it *)
+Definition closed_row (o : hypothesis) (u : str) : Prop :=
+    forall v, In v o.(V) ->
+        cell o u v = true <->
+        exists u', In u' o.(U) /\ prime o u' /\ covered o u' u /\ cell o u' v = true.
+
+Lemma closed_row_dec : forall o u, {closed_row o u} + {~ closed_row o u}.
+Proof.
+    intros. unfold closed_row.
+    induction (V o).
+        left. intros. destruct H.
+    assert (Pdec : {exists u', In u' o.(U) /\ prime o u' /\ covered o u' u /\ cell o u' a = true}
+                 + {~ exists u', In u' o.(U) /\ prime o u' /\ covered o u' u /\ cell o u' a = true}).
+    { clear IHl.
+        induction (U o).
+            right. intro Contra. destruct Contra, H. inversion H.
+        destruct (prime_dec o a0).
+        - destruct (covered_dec o a0 u).
+          + destruct (Bool.bool_dec (cell o a0 a) true).
+              left. exists a0. intuition.
+            destruct IHl0.
+              left. destruct e. exists x. split; [now right | intuition].
+            right. intro Contra. destruct Contra, H, H0, H1, H.
+              now subst.
+            apply n0. eauto.
+          + destruct IHl0.
+              left. destruct e. exists x. split; [now right | intuition].
+            right. intro Contra. destruct Contra, H, H0, H1, H.
+              now subst.
+            apply n0. eauto.
+        - destruct IHl0.
+            left. destruct e. exists x. split; [now right | intuition].
+          right. intro Contra. destruct Contra, H, H0, H.
+            now subst.
+          apply n0. eauto.
+    }
+    destruct (Bool.bool_dec (cell o u a) true).
+    - destruct Pdec.
+      + destruct IHl.
+            left. intros. destruct H; [subst; now split | auto].
+        right. intro. apply n. intros. apply H. now right.
+      + right. intro. apply n. now apply (proj1 (H a (or_introl eq_refl))).
+    - destruct Pdec.
+        right. intro. apply n. now apply (proj2 (H a (or_introl eq_refl))).
+      destruct IHl.
+        left. intros. destruct H.
+            subst. intuition.
+        now apply i.
+      right. intro. apply n1. intros. apply H. now right.
+Defined.
+
+Definition closed (o : hypothesis) : Prop :=
+    forall u, In u (USigma o) -> closed_row o u.
+
+Lemma closed_dec : forall o,
+    closed o + {u : str | In u (USigma o) /\ ~ closed_row o u}.
+Proof.
+    intros. unfold closed.
+    induction (USigma o).
+        left. intros. destruct H.
+    destruct (closed_row_dec o a).
+    - destruct IHl.
+        left. intros. destruct H; auto; now subst.
+      right. destruct s. exists x. split; [now right | intuition].
+    - right. exists a. split; [now left | assumption].
+Defined.
+
+(* Definition 9 *)
+(** A table is RFSA-consistent if for all u, u' \in U, a \in S,
+    row(u') covered by row(u) -> row(u'a) covered by row(ua). *)
+Definition rfsa_consistent (o : hypothesis) : Prop :=
+    forall u u' a,
+        In u o.(U) -> In u' o.(U) -> In a enum ->
+        covered o u u' -> covered o (u ++ [a]) (u' ++ [a]).
+
+Lemma consistent_triple_dec : forall o u u' a,
+    {covered o u u' -> covered o (u ++ [a]) (u' ++ [a])} +
+    {~ (covered o u u' -> covered o (u ++ [a]) (u' ++ [a]))}.
+Proof.
+    intros. destruct (covered_dec o u u').
+    - destruct (covered_dec o (u ++ [a]) (u' ++ [a])).
+        left. now intros.
+      right. intro Contra. auto.
+    - left. now intros.
+Defined.
+
+Lemma consistent_row_a_dec : forall o u a (us : list str),
+    (forall u', In u' us -> covered o u u' -> covered o (u ++ [a]) (u' ++ [a]))
+    + {u' : str | In u' us /\ ~ (covered o u u' -> covered o (u ++ [a]) (u' ++ [a]))}.
+Proof.
+    intros. induction us.
+        left. intros. destruct H.
+    destruct (consistent_triple_dec o u a0 a).
+    - destruct IHus.
+        left. intros. destruct H; subst; auto.
+      right. destruct s. exists x. intuition.
+    - right. exists a0. intuition.
+Defined.
+
+Lemma consistent_row_dec : forall o u (us : list str),
+    (forall u' a, In u' us -> In a enum -> covered o u u' -> covered o (u ++ [a]) (u' ++ [a]))
+    + {p : str * s.t | let '(u', a) := p in
+        In u' us /\ In a enum /\ ~ (covered o u u' -> covered o (u ++ [a]) (u' ++ [a]))}.
+Proof.
+    intros. induction enum.
+        left. intros. destruct H0.
+    destruct (consistent_row_a_dec o u a us).
+    - destruct IHl.
+        left. intros. destruct H0; subst; auto.
+      right. destruct s, x. exists (s, t0). intuition.
+    - right. destruct s, a0. exists (x, a). intuition.
+Defined.
+
+Lemma consistent_outer_dec : forall o (us : list str),
+    (forall u u' a, In u us -> In u' o.(U) -> In a enum -> covered o u u' -> covered o (u ++ [a]) (u' ++ [a]))
+    + {p : str * str * s.t | let '(u, u', a) := p in
+        In u us /\ In u' o.(U) /\ In a enum /\ ~ (covered o u u' -> covered o (u ++ [a]) (u' ++ [a]))}.
+Proof.
+    intros. induction us.
+        left. intros. destruct H.
+    destruct (consistent_row_dec o a (U o)).
+    - destruct IHus.
+        left. intros. destruct H; subst; auto.
+      right. destruct s, x, p. exists (s, s0, t0). intuition.
+    - right. destruct s, x. exists (a, s, t0). intuition.
+Defined.
+
+Lemma rfsa_consistent_dec : forall o,
+    rfsa_consistent o
+    + {p : str * str * s.t | let '(u, u', a) := p in
+        In u o.(U) /\ In u' o.(U) /\ In a enum /\ ~ (covered o u u' -> covered o (u ++ [a]) (u' ++ [a]))}.
+Proof.
+    intros. unfold rfsa_consistent.
+    destruct (consistent_outer_dec o (U o)); auto.
+Defined.
+
+(* Definition 10 *)
+Definition make_rfsa (o : hypothesis) : N.t { q | memr o q = true }.
+    set (state := { q | memr o q = true }).
+    assert (initial : list state). {
+        refine (list_with_proof (cover_set o []) (fun q => memr o q = true) _).
+        intros x Hx. now apply (cover_set_memr o []). }
+    assert (transition : state -> s.t -> list state). {
+        intros q a.
+        refine (list_with_proof (cover_set o (proj1_sig q ++ [a]))
+                  (fun q' => memr o q' = true) _).
+        intros x Hx. now apply (cover_set_memr o (proj1_sig q ++ [a])). }
+    set (accept := fun (q : state) => o.(T) (proj1_sig q)).
+    assert (mempf : forall x, In x (prime_reps o) -> memr o x = true)
+        by (intros x Hx; now apply mem_In).
+    set (ls := list_with_proof (prime_reps o) (fun q => memr o q = true) mempf).
+    refine {| initial    := initial;
+              transition := transition;
+              accept     := accept;
+              states     := ls;
+              states_complete := _ |}.
+    intros w q Hq.
+    assert (Hin : In (proj1_sig q) (prime_reps o))
+        by apply (mem_In str_eq), (proj2_sig q).
+    assert (Heq : q = exist _ (proj1_sig q) (mempf (proj1_sig q) Hin)). {
+        destruct q as (q' & Hq'); simpl.
+        f_equal. apply (UIP_dec Bool.bool_dec). }
+    rewrite Heq.
+    apply (list_with_proof_complete (prime_reps o) (fun q => memr o q = true)).
+    intros. apply UIP_dec, Bool.bool_dec.
+Defined.
+
+End NLstar.
