theories/SetLemmas.v
@@ -1,0 +1,98 @@
+From Stdlib Require Import List.
+
+Section SL.
+
+Variable X : Type.
+Variable eq_dec : forall (x y : X), {x = y} + {x <> y}.
+
+Definition finite (f : X -> bool) :=
+    {l : list X | NoDup l /\
+        forall (s : X), f s = true <-> In s l}.
+
+Definition num_states_of_fin {f : X -> bool} (H : finite f) : nat :=
+    match H with
+    | exist _ x _ => List.length x
+    end.
+
+(** Updating sets *)
+Definition update (S : X -> bool) k b :=
+    fun s => if eq_dec s k then b else S s.
+
+Notation "s [ k := v ]" := (update s k v).
+
+Lemma update_neq : forall S x y k,
+    x <> y ->
+    S[x := k] y = S y.
+Proof.
+    intros. unfold update.
+    destruct eq_dec; now subst.
+Qed.
+
+Lemma update_eq : forall S x k,
+    S[x := k] x = k.
+Proof.
+    intros. unfold update.
+    destruct eq_dec; now subst.
+Qed.
+
+Lemma finite_subset_is_smaller : forall
+    (f g : X -> bool)
+    (FinF : finite f)
+    (FinG : finite g)
+    (FsubG : forall (x : X), f x = true -> g x = true),
+    num_states_of_fin FinF <= num_states_of_fin FinG.
+Proof.
+    intros. destruct FinF as (fl & NDF & InF),
+                     FinG as (gl & NDG & InG).
+    simpl.
+    apply NoDup_incl_length.
+        assumption.
+    unfold incl. intros x Hx.
+    now apply (proj1 (InG x)), FsubG, (proj2 (InF x)).
+Qed.
+
+Lemma finite_update_impl_finite : forall
+    (f : X -> bool) k v
+    (FinUpdF : finite f[k := v]),
+    finite f.
+Proof.
+    intros. destruct FinUpdF as (fl' & NDfl' & Infl).
+    unfold finite, update in *.
+    destruct v, (f k) eqn:Hfk.
+    - exists fl'. split. assumption.
+        intro s. specialize (Infl s). destruct (eq_dec s k).
+            subst. now rewrite Hfk.
+        assumption.
+    - exists (filter f fl'). split.
+        + clear Infl. induction fl' as [| h t IH].
+            constructor.
+          inversion NDfl'; subst. simpl. destruct (f h) eqn:Hfh.
+            constructor.
+                intro C. apply filter_In in C.
+                now destruct C.
+            now apply IH.
+          now apply IH.
+        + intro s. specialize (Infl s). rewrite filter_In. 
+            destruct (eq_dec s k) as [e|n].
+                subst. rewrite Hfk. now split; intro H.
+            split; intro H.
+                split; [now apply Infl | assumption].
+            now destruct H.
+    - exists (k :: fl'). split.
+        + constructor; auto.
+          intro C. specialize (Infl k). destruct (eq_dec k k).
+            now rewrite <- Infl in C.
+          contradiction.
+        + intro s. specialize (Infl s). simpl. destruct (eq_dec s k).
+            subst. rewrite Hfk. split; auto.
+            split; intro H.
+                right. now apply Infl.
+            destruct H as [e2 | Hfl]; intuition.
+    - exists fl'. split; auto.
+        intro s. specialize (Infl s). destruct (eq_dec s k).
+            subst. now rewrite Hfk.
+            assumption.
+Defined.
+
+End SL.
+
